Examples.lean
@@ -1,7 +1,9 @@
+import Examples.BR93
 import Examples.ElGamal
 import Examples.FrankingProtocol
 import Examples.HashedElGamal
 import Examples.OneTimePad
+import Examples.PRGfromPRF
 import Examples.Pedersen
 import Examples.RF_RP_Switching_alt
 import Examples.Regev
